better netkat tactics; make instances global

Classes.v
@@ -11,50 +11,45 @@ Generalizable Variables X Y.
 
 Section Equality_Type.
 
-Class eqType (X : Type) : Type := eq_dec : forall x y : X, {x=y} + {x<>y}.
+Class EqType (X : Type) : Type := eq_dec : forall x y : X, {x=y} + {x<>y}.
 
-Definition eqb `{eqType X} (x y : X) := if eq_dec x y then true else false.
+Definition eqb `{EqType X} (x y : X) := if eq_dec x y then true else false.
 
-Theorem eqb_eq `{eqType X} (x y : X) : eqb x y = true <-> x=y.
+Theorem eqb_eq `{EqType X} (x y : X) : eqb x y = true <-> x=y.
 Proof. unfold eqb. destruct (eq_dec x y); intuition. inversion H0. Qed.
 
-Theorem eqb_eq_false `{eqType X} (x y : X) : eqb x y = false <-> x<>y.
+Theorem eqb_eq_false `{EqType X} (x y : X) : eqb x y = false <-> x<>y.
 Proof. unfold eqb. destruct (eq_dec x y); intuition. Qed.
 
 Hint Resolve eqb_eq eqb_eq_false.
 
-Instance : eqType bool := bool_dec.
-Instance : eqType nat := eq_nat_dec.
-Program Instance : eqType True := fun x y => match x,y with I,I => left _ end. 
-Program Instance : eqType False := fun x y => match x,y with end.
+Global Instance : EqType bool := bool_dec.
+Global Instance : EqType nat := eq_nat_dec.
+Global Program Instance : EqType True := fun x y => match x,y with I,I => left _ end. 
+Global Program Instance : EqType False := fun x y => match x,y with end.
 
-Program Instance sum_eqType `(eqType X) `(eqType Y) : eqType(X+Y) := fun a b =>
-match a, b with
+Global Program Instance sum_EqType `(EqType X) `(EqType Y) : EqType(X+Y) :=
+fun a b =>
+  match a, b with
   | inl _, inr _ | inr _, inl _ => right _
-  | inl z, inl z' | inr z, inr z' =>
-      match eq_dec z z' with left _ => left _
-                           | right _ => right _
-      end
-end.
+  | inl z, inl z' | inr z, inr z' => if eq_dec z z' then left _ else right _ 
+  end.
 
-Program Instance prod_eqType `(eqType X) `(eqType Y) : eqType(X*Y) := fun a b =>
-match a,b with
+Global Program Instance prod_EqType `(EqType X) `(EqType Y) : EqType(X*Y) :=
+fun a b =>
+  match a,b with
   | pair x y, pair x' y' =>
-  match eq_dec x x', eq_dec y y' with
-    | left _, left _ => left _
-    | left _, right _ | right _, left _ | right _, right _ => right _
-  end
-end.
+    if eq_dec x x' then (if eq_dec y y' then left _ else right _)
+    else right _
+  end.
 
-Program Instance list_eqType `(eqType X) : eqType(list X) := fix f xs ys :=
+Global Program Instance list_EqType `{EqType X} : EqType(list X) := fix f xs ys :=
 match xs, ys with
   | nil, nil => left _
   | nil,cons _ _ | cons _ _,nil => right _
   | cons x xs, cons y ys =>
-    match eq_dec x y with
-      | left _ => match f xs ys with left _ => left _ | right _ => right _ end
-      | right _ => right _
-    end
+    if eq_dec x y then (if f xs ys then left _ else right _)
+    else right _
 end.
 
 Eval compute in eqb 
@@ -63,6 +58,8 @@ Eval compute in eqb
 
 End Equality_Type.
 
+Definition test := (@eqb (list (prod bool nat)) _).
+Recursive Extraction test.
 
 
 
@@ -75,30 +72,28 @@ Class Finite (X : Type) : Type := enum : {xs: list X|forall x, In x xs}.
 Definition enum' X `{Finite X} := proj1_sig enum.
 Hint Unfold enum'.
 
-Program Instance : Finite bool := [true;false].
-Next Obligation. destruct x; intuition. Qed.
+Global Program Instance : Finite bool := [true;false].
+Next Obligation. destruct x; intuition. Defined.
 
-Program Instance : Finite True := [I].
-Next Obligation. destruct x; intuition. Qed.
+Global Program Instance : Finite True := [I].
+Next Obligation. destruct x; intuition. Defined.
 
-Program Instance : Finite False := [].
+Global Program Instance : Finite False := [].
 
-Check @enum.
-
-Program Instance sum_finite `(p1:Finite X) `(p2:Finite Y) : Finite(X+Y) :=
-  (map (@inl X Y) (@enum X p1)) ++ (map (@inr X Y) (@enum Y p2)).
+Global Program Instance sum_finite `(p1:Finite X) `(p2:Finite Y) : Finite(X+Y) :=
+  (map (@inl X Y) enum) ++ (map (@inr X Y) enum).
 Next Obligation.
   destruct (@enum X p1) as [xs px]; destruct (@enum Y p2) as [ys py]; simpl.
   apply in_or_app.
-  destruct x; [left|right]; apply in_map; auto.
-Qed.
+  destruct x; [left|right]; auto using in_map.
+Defined.
 
-Program Instance prod_finite `(px: Finite X) `(py: Finite Y) : Finite(X*Y) :=
+Global Program Instance prod_finite `(px: Finite X) `(py: Finite Y) : Finite(X*Y) :=
   list_prod enum enum.
 Next Obligation.
   destruct (@enum X px) as [xs p1]; destruct (@enum Y py) as [ys p2]; simpl.
   auto using in_prod.
-Qed.
+Defined.
 
 
 
@@ -111,7 +106,8 @@ match xs with
   | x::xs => x :: (map (weaken x) (siglist xs))
 end.
 
-Program Instance fin_of_list {X} (xs : list X) : Finite {x|In x xs} := siglist xs.
+Global Program Instance fin_of_list {X} (xs : list X) : Finite {x|In x xs} := 
+  siglist xs.
 Next Obligation.
   induction xs; destruct H.
   + subst a. simpl. auto.
@@ -121,7 +117,7 @@ Next Obligation.
     by auto.
     rewrite <- H.
     apply in_map. auto.
-Qed.
+Defined.
 
 End Finite_Of_List.
 
@@ -135,90 +131,40 @@ End Finite.
 
 Section Finite_Functions.
 
-Definition eq_dec_f `{Finite X} `{eqType (list Y)} (f g : X->Y) :=
+Definition eq_dec_f `{Finite X} `{EqType Y} (f g : X->Y) :=
   eq_dec (map f (enum' X)) (map g (enum' X)).
 
-Program Instance fun_eqType `(Finite X) `(p:eqType Y) : eqType (X->Y) := fun f g =>
-  if @eq_dec_f X _ Y (list_eqType p) f g then left _ else right _.
+Global Program Instance fun_EqType `(Finite X) `(EqType Y) : EqType (X->Y) := 
+  fun f g => if eq_dec_f f g then left _ else right _.
 Next Obligation.
   extensionality x.
   assert(In x (enum' X)) by (unfold enum'; destruct enum; auto).
-  induction enum'; simpl in *; inversion H0; clear H0; intuition. 
+  induction enum'; simpl in *; inversion H1; clear H1; intuition.
   subst a; assumption.
-Qed.
-Next Obligation. intro eq; subst; apply H0; reflexivity. Qed.
+Defined.
+Next Obligation. intro eq; apply H1; congruence. Defined.
 
-Definition functs' `(Finite X) `(Finite Y) : list (X->Y) := (fix loop ys :=
-match ys with
-  | [] => []
-  | y::ys => (fun _ => y) :: (loop ys)
-end) (enum' Y).
+Definition functs `(Finite X) `(Finite Y) `{EqType X} : list(X->Y) :=
+  fold_left 
+    (fun fs x => flat_map (fun f => 
+      map (fun y x' => if eq_dec x x' then y else f x') (enum' Y)) fs)
+    (enum' X)
+    (map (fun y => fun _ => y) (enum' Y)).
 
-Fixpoint functs `(px:Finite X) `{_:eqType X} `(py:Finite Y) : list (X->Y) := 
-(fix loop xs :=
-  match xs with
-    | [] => functs' px py
-    | x::xs => flat_map (fun f => map (fun y x' => if eq_dec x x' then y else f x') (enum' Y))
-       (loop xs)
-  end) (enum' X).
+Definition test `(Finite X) `(Finite Y) (y:Y) :=
+  (fun (x:X) => match x with end).
 
-Instance fun_finite `(Finite X) `(Finite Y) : Finite(X->Y) := fun f g =>
+Program Instance fun_finite `(px:Finite X) `(py:Finite Y) `{_:EqType X} `{_:EqType Y} 
+: Finite(X->Y) :=
+  functs px py.
+Next Obligation.
+  rename x into f.
+  unfold functs.
+  induction (enum' X); simpl in *.
+  functional induction
+  assert(xs := enum' X).
+  induction (xs).
 
 
 
 End Finite_Functions.
-
-
-
-
-
-
-
-Fixpoint power {X} (xs : list X) :=
-match xs with
-  | [] => [[]]
-  | x::xs => 
-   map (fun p => app (fst p) (snd p)) (list_prod [[x];[]] (power xs))
-end.
-
-Definition insertn {X} (n:nat) (x:X) (xs:list X) := app (firstn n xs) (x::skipn n xs).
-
-
-Lemma in_insertn X (x:X) y n xs : 
-  In x xs \/ x=y -> In x (insertn n y xs).
-Proof.
-  intro H.
-  unfold insertn. apply in_or_app.
-  destruct H as [H|H].
-  + rewrite <- (firstn_skipn n) in H. apply in_app_or in H.
-    destruct H; [left|right]; simpl; auto.
-  + right. simpl. auto.
-Qed.
-
-Fixpoint power {X} (xs : list X) :=
-match xs with
-  | [] => [[]]
-  | x::xs => flat_map f (power xs)
-
-Lemma in_power
-
-Program Instance list_finite `(p: Finite X) : Finite(list X) :=
-
-End Finite.
-
-Check Finite (sum (prod bool True) False).
-
-
-Class FinTy : Type := {
-  T :> Type;
-  T_finite :> Finite T
-}.
-
-Definition test `(FinTy) := enum.
-
-Check test.
-
-Parameter X : FinTy.
-
-Check T.
-Check @enum X.
